Normalized_Zone_Semantics_Certification_Impl.thy
@@ -816,6 +816,11 @@ proof -
     by auto
 qed
 
+context
+  fixes splitteri :: "'si list \<Rightarrow> 'si list list"
+  assumes full_split: "set xs = (\<Union>xs \<in> set (splitteri xs). set xs)"
+begin
+
 interpretation Reachability_Impl_imp_to_pure
   where A = "mtx_assn n"
     and F = F
@@ -868,6 +873,8 @@ interpretation Reachability_Impl_imp_to_pure
     by (rule right_unique_location_rel)
   subgoal
     using left_unique_location_rel unfolding IS_LEFT_UNIQUE_def .
+  subgoal
+    using full_split .
   done
 
 concrete_definition certify_unreachable_pure
@@ -877,6 +884,8 @@ lemma certify_unreachable_pure_refine:
   assumes "fst ` set M_list = set L_list" certify_unreachable_pure
   shows "\<nexists>u l' u'. (\<forall>c\<le>n. u c = 0) \<and> conv_A A \<turnstile>' \<langle>l\<^sub>0, u\<rangle> \<rightarrow>* \<langle>l', u'\<rangle> \<and> F' (l', u')"
   using certify_unreachable_pure.refine[OF L_dom_M_eqI] assms op_precise_unreachable_correct by simp
+
+end
 
 thm
   certify_unreachable_impl.refine[
@@ -1046,20 +1055,17 @@ lemma deadlock_unreachability_checker3_hnr:
   fixes P_loc :: "'si \<Rightarrow> bool"
     and L_list :: "'si list"
     and M_list :: "('si \<times> int DBMEntry list list) list"
-  fixes splitter :: "'s list \<Rightarrow> 's list list" and splitteri :: "'si list \<Rightarrow> 'si list list"
+  fixes splitteri :: "'si list \<Rightarrow> 'si list list"
   assumes "\<And>li. P_loc li \<Longrightarrow> \<exists>l. (li, l) \<in> loc_rel"
     and "list_all (\<lambda>x. P_loc x \<and> states_mem_impl x) L_list"
     and "list_all (\<lambda>(l, xs). list_all (\<lambda>M. length M = Suc n * Suc n) xs) M_list"
     and "fst ` set M_list = set L_list"
-  assumes full_split: "\<And>xs. set xs = (\<Union>xs \<in> set (splitter xs). set xs)"
-    and same_split:
-    "\<And>L Li.
-      list_assn (list_assn location_assn) (splitter L) (splitteri Li) = list_assn location_assn L Li"
+  assumes full_split: "\<And>xs. set xs = (\<Union>xs \<in> set (splitteri xs). set xs)"
   shows
-    "deadlock.certify_unreachable_pure L_list M_list
+    "deadlock.certify_unreachable_pure L_list M_list splitteri
     \<longrightarrow> (\<forall>u. (\<forall>c\<le>n. u c = 0) \<longrightarrow> \<not> deadlock (l\<^sub>0, u))"
   using deadlock.certify_unreachable_pure_refine[
-      OF assms(1-2) assms(4)[THEN equalityD1] assms(3) assms(4)
+      OF assms(1-2) assms(4)[THEN equalityD1] assms(3) full_split assms(4)
       ]
   unfolding deadlock_def steps'_iff[symmetric] by auto
 
