Simple_Networks/Simple_Network_Language_Certificate_Checking.thy
@@ -289,10 +289,11 @@ theorem unreachability_checker3_refine:
     and "fst ` set M_list = set L_list"
     and "formula = formula.EX \<phi>"
   shows "
-  impl.certify_unreachable_pure L_list M_list \<longrightarrow>
+  impl.certify_unreachable_pure L_list M_list (split_k num_split) \<longrightarrow>
     \<not> Simple_Network_Language.conv A,(L\<^sub>0, map_of s\<^sub>0, \<lambda>_. 0) \<Turnstile> formula"
   using impl.certify_unreachable_pure_refine[
-      OF state_impl_abstract', OF assms(1,2) assms(4)[THEN equalityD1] assms(3,4)
+      OF state_impl_abstract', OF assms(1,2) assms(4)[THEN equalityD1] assms(3)
+         split_k_full_split assms(4)
       ]
     unreachability_prod[OF assms(5)]
   by auto
@@ -402,7 +403,9 @@ lemma no_deadlock_certifier_alt_def1:
     Heap_Monad.return r
   }"
   unfolding no_deadlock_certifier_def
-  by (subst impl.deadlock_unreachability_checker_alt_def[OF state_impl_abstract', OF _ A assms(2,3) split_k_full_split list_assn_split];
+  by (subst impl.deadlock_unreachability_checker_alt_def[
+        OF state_impl_abstract', OF _ A assms(2,3) split_k_full_split list_assn_split
+        ];
       simp)
 
 schematic_goal check_deadlock_impl_alt_def:
@@ -531,9 +534,9 @@ lemmas no_deadlock_certifier2_refine' =
   ]
 
 schematic_goal unreachability_checker3_alt_def:
-  "impl.certify_unreachable_pure L_list M_list \<equiv> ?x"
+  "impl.certify_unreachable_pure L_list M_list (split_k num_split) \<equiv> ?x"
   apply (subst impl.certify_unreachable_pure_def[
-      OF state_impl_abstract', OF _ A assms(2,3)
+      OF state_impl_abstract', OF _ A assms(2,3) split_k_full_split
       ], (simp; fail))
   apply (abstract_let "impl.Mi M_list" Mi)
   apply (subst impl.Mi_def[OF state_impl_abstract', of states'_memi, OF _ A assms(2,3)])
@@ -563,10 +566,10 @@ definition no_deadlock_certifier3 where
     states'_memi (\<lambda>(l, M). impl.check_deadlock_impl l M \<bind> (\<lambda>r. Heap_Monad.return (\<not> r)))"
 
 schematic_goal no_deadlock_certifier3_alt_def:
-  "no_deadlock_certifier3 L_list M_list \<equiv> ?x"
+  "no_deadlock_certifier3 L_list M_list (split_k num_split) \<equiv> ?x"
   unfolding no_deadlock_certifier3_def
   apply (subst impl.deadlock_unreachability_checker3_def[
-        OF state_impl_abstract', OF _ A assms(2,3)
+        OF state_impl_abstract', OF _ A assms(2,3) split_k_full_split
         ], (simp; fail))
   apply (abstract_let "impl.Mi M_list" Mi)
   apply (subst impl.Mi_def[OF state_impl_abstract', of states'_memi, OF _ A assms(2,3)])
@@ -592,7 +595,7 @@ schematic_goal no_deadlock_certifier3_alt_def:
 lemmas no_deadlock_certifier3_refine' =
   impl.deadlock_unreachability_checker3_hnr[
     folded no_deadlock_certifier3_def,
-    OF state_impl_abstract' A assms(3) _ split_k_full_split list_assn_split
+    OF state_impl_abstract' A assms(3) _ split_k_full_split
   ]
 
 end (* Anonymous context *)
@@ -632,7 +635,7 @@ theorem no_deadlock_certifier3_refine:
   assumes "list_all states'_memi L_list"
       and "list_all (\<lambda>(l, y). list_all (\<lambda>M. length M = Suc m * Suc m) y) M_list"
       and "fst ` set M_list = set L_list"
-  shows "no_deadlock_certifier3 L_list M_list \<longrightarrow>
+  shows "no_deadlock_certifier3 L_list M_list (split_k num_split) \<longrightarrow>
     \<not> has_deadlock (Simple_Network_Language.conv A) (L\<^sub>0, map_of s\<^sub>0, \<lambda>_. 0)"
   using no_deadlock_certifier3_refine' assms unfolding deadlock_prod[symmetric] by auto
 
@@ -884,10 +887,10 @@ definition
   in if check then
     if dc then
         no_deadlock_certifier3
-          broadcast bounds' automata m num_states num_actions L\<^sub>0 s\<^sub>0 L_list M_list
+          broadcast bounds' automata m num_states num_actions L\<^sub>0 s\<^sub>0 L_list M_list num_split
       else
         unreachability_checker3
-          broadcast bounds' automata m num_states num_actions L\<^sub>0 s\<^sub>0 formula L_list M_list
+          broadcast bounds' automata m num_states num_actions L\<^sub>0 s\<^sub>0 formula L_list M_list num_split
   else False"
 
 definition
